# 3940 AS 02

## Main

### Question 1

#### (a) From Descartes’s rule of signs, conclude that the equation $𝑥^{2𝑛} − 1 = 0$ has $2n−2$ imaginary roots. 

$$
f(-x) = (-x)^{2n} - 1 = x^{2n} - 1 = 0 \,\,\text{Sign Has Changed Once}
$$

So, $f(x) = 0$ has one negative real root, that is $-1$.

Also, $f(x) = 0$ has one positive real root $x = 1$ ($f(x)$ is symmetric about the y-axis)

Since the equation has two real roots, the number of imaginary roots is $2n-2$

#### (ii) Without actually obtaining the roots, show that $𝑥^6 − 5𝑥^5 − 7𝑥^2 + 8𝑥 + 20 = 0$ possess imaginary roots. 

From Descartes’s rule of signs, since there are 2 sign changed for $f(x) = 0$. So, the equation has 2 positive real roots.

Similarly, since there are 2 sign changed for $f(-x) = x^6 + 5x^5 - 7x^2 -8x + 20 = 0$, so the equation has 2 negative real roots.

Since the degree of $f(x)$ is $6$, which means $f(x)$ has 6 roots.

Hence, the equation $f(x) = 0$ has two imaginary roots. 

### Question 2

The equation $𝑓(𝑥) = 𝑥^2 − 2𝑒^𝑥 = 0$ has a solution in the interval [−1,1].

#### (a) With $p_0 = -1$ and $p_1 = 1$, calculate $p_2$ using the Secant method.

From Secant method,
$$
\begin{aligned}
x_2 &= x_1 - \frac{f(x_1)}{\frac{f(x_1)  -f(x_0)}{x_1-x_0}} \\
&= \frac{x_0f(x_1)-x_1f(x_0)}{f(x_1)  -f(x_0)}
\end{aligned}
$$
Since
$$
f(-1) = (-1)^2 - 2e^{-1} = 1 - \frac{2}{e} \\
f(1) = 1^2 - 2e^{1} = 1 - 2e
$$
So,
$$
\begin{aligned}
x_2 = \frac{-2+2e+\frac{2}{e}}{\frac{2}{e}  -2e} \approx -0.8876
\end{aligned}
$$

#### (b) With $p_2$ from part (a), calculate $p_3$ using the Newton's method.

From the Newton's method,
$$
\begin{aligned}
x_{n+1} &= x_n - \frac{f(x_n)}{f'(x_n)} \\
\therefore x_3 &= x_2 - \frac{f(x_2)}{f'(x_2)} \\
\end{aligned}
$$
Since,
$$
f'(x) = 2x - 2e^x
$$
The value of $f(p_2)$ and $f'(p_2)$ could be calculated as below,
$$
f(-0.8876) = (-0.8876)^2 - 2e^{-0.8876} \approx -0.03543 \\
f'(-0.8876) = 2(-0.8876) - 2e^{-0.8876} \approx -2.59856 \\
$$
Therefore,
$$
x_3 = -0.8876 - \frac{-0.03543}{-2.59856} = -0.90123
$$

### Question 3

The equation $𝑓(𝑥) = 2 − 𝑥^2 \sin 𝑥 = 0$ has a solution in the interval [−1,2].

#### (a)  Verify that the Bisection method can be applied to the function $𝑓(𝑥)$ on [−1,2].

$$
f(-1) = 2 - \sin(-1) = 2.814 > 0 \\
f(2) = 2 - 2^2\sin(2) = -1.6368 < 0 \\
$$

So $f(-1)f(2) > 0$

Therefore, the equation has a solution in the interval $[-1,2]$, and the Bisection method can be applied to the function $f(x)$

#### (b) Using the error formula for the Bisection method, find the number of iterations needed for accuracy $10^{−7}$

The error formula for the Bisection method is $n\geq \frac{\log(b-a)-\log \sigma}{\log 2}$ where $[a,b] = [-1,2], \sigma = 10^{-7}$

So,
$$
n \geq \frac{\log(2+1) - \log 10^{-6}}{\log 2} = \frac{\log(3) +7}{\log 2} \geq 24.8
$$
Therefore, the number of iterations needed for accuracy $10^{-7}$ is $25$

#### (c) Compute $p_3$ for the Bisection method

$$
\begin{aligned}
p_0 &= f(0.5) = 2 - 0.5^2\sin(0.5) \approx 1.88015 > 0 \\
p_1 &= \frac{0.5 + 2}{2} = 1.25 \\
f(p_1) &= f(1.25) = 2 - 1.25^2\sin(1.25) > 0 \\
p_2 &= \frac{1.25 + 2}{2} = 1.625 \\
f(p_2) &= f(1.625) = 2 - 1.625^2\sin(1.625) \approx -0.64 < 0 \\
\therefore p_3 &= \frac{1.25 + 1.625}{2} = 1.4375
\end{aligned}
$$



### Question 4

The following refer to the fixed-point problem:

#### (a)  State the theorem which gives conditions for a fixed-point sequence to converge to a unique fixed point.

If $g(x) = x_{n+1}$, theorem state that $|g'(x)| < 1$ then sequence is converge to fixed point.

#### (b) Given $g(x) = \frac{2-x^3 + 2x}{3}$, use the theorem to show that the fixed-point sequence will converge to unique fixed-point of $g(x)$ for any $p_0$ in $[-1,1.1]$.

From the question, we have $g'(x)$,
$$
g'(x) = \frac{-3x^2+2}{3} = -x^2 + \frac{2}{3}
$$
Since $|g'(0)| = \frac{2}{3} < 1$, $|g'(1)| = \frac{1}{3} < 1$,

Sequence is converge to fixed point.

#### (c) With $p_0 = 0.5$ generate $p_3$

$$
x_{x+1} = \frac{2 - x_n^3 + 2x_n}{3},\,x_0 = 0.5
$$

$$
\begin{aligned}
p_1 &= \frac{2-0.5^3 + 2\times 0.5}{3} \approx 0.9583 \\
p_2 &= \frac{2-0.9583^3 + 2\times 0.9583}{3} \approx 1.0122 \\
p_3 &= \frac{2-1.0122^3 + 2\times1.0122}{3} \approx 0.9957\\
\end{aligned}
$$

Therefore, $p_3 = 0.9957$

### Question 5

What is the main difference between secant and regula falsi method? Compute the root of the equation $𝑥^2𝑒^{−𝑥/2} = 1$ in the interval $[0, 2]$ correct to three decimal places using both secant method and regula falsi method.

#### Solution

The regula falsi is a bracketing algorithm. It iterates through intervals that always contain a root whereas the secant method is basically Newton's method without explicitly computing the derivative at each iteration. The secant is faster but may not converge at all.

Given equation $𝑓(𝑥) = 𝑥^2 𝑒^{-𝑥/2} - 1 = 0$ has a solution in the interval $[0,2]$

##### using the Secant method

From Secant method,
$$
\begin{aligned}
x_2 &= x_1 - \frac{f(x_1)}{\frac{f(x_1)  -f(x_0)}{x_1-x_0}} \\
&= \frac{x_0f(x_1)-x_1f(x_0)}{f(x_1)  -f(x_0)}
\end{aligned}
$$
Since
$$
f(0) = -1 \\
f(2) = 2^2e^{-1} - 1 = \frac{4}{e} - 1 \\
$$
So,
$$
\begin{aligned}
x_2 = \frac{2}{\frac{4}{e}} = \frac{e}{2} \approx 1.359
\end{aligned}
$$

##### using the Newton's method.

From the Newton's method,
$$
\begin{aligned}
x_{n+1} &= x_n - \frac{f(x_n)}{f'(x_n)} \\
\end{aligned}
$$
Since,
$$
f'(x) = 2𝑥 𝑒^{-𝑥/2} -\frac{1}{2} x^2e^{-x/2}
$$
The value of $f(x_1)$ and $f'(x_1)$ could be calculated as below,
$$
f(2) = \frac{4}{e} - 1 \\
f'(2) = \frac{4}{e}-\frac{2}{e} = \frac{2}{e} \\
$$
Therefore,
$$
x_2 = 2-\frac{\frac{4}{e} - 1}{\frac{2}{e}} = 2 - \frac{4-e}{2} = \frac{e}{2} \approx 1.359
$$

### 

### Question 6

#### (a) Suppose the function $𝑓(𝑥)$ has a unique zero $p$ in the interval $[a, b]$. Further, suppose $𝑓′′(𝑥)$ exists and is continuous on the interval $[a, b]$. Under what conditions, Newton’s method give a quadratically convergent sequence to $p$? 

From the Newton's method,
$$
\begin{aligned}
x_{n+1} &= x_n - \frac{f(x_n)}{f'(x_n)} = g(x_n)\\
\end{aligned}
$$
Since $r$ is a root of $f(x) = 0$, $r=g(r)$, so we have
$$
\begin{aligned}
x_{n+1} - r &= g(x_n) - g(r) \\
&= g(r) + g'(r)(x_n-r) + \frac{g''(\xi)}{2}(x_n - r)^2 - g(r) \\
&= g'(r)(x_n-r) + \frac{g''(\xi)}{2}(x_n - r)^2
\end{aligned}
$$
where $\xi$ lies in the interval $[x_n, r]$

Since
$$
g'(r) = \frac{f(r)f'''(r)}{[f'(r)]^2} = 0, \, f(r) = 0
$$
we have
$$
(x_{n+1} - r) = \frac{g''(\xi)}{2}(x_n - r)^2, \, \text{where r is a constant}
$$
Therefore, Newton’s method give a quadratically convergent sequence to $p$.

#### (b) Using Newton’s method, construct an iterative formula to find $\sqrt[\leftroot{-2}k]{N}$$^k\sqrt{𝑁}$ 𝑘 i.e. $k^{th}$ root of any number $N$. 

Given

$f(x) = \sqrt[\leftroot{-2}k]{x} = x^{1/k}$

By the Newton's method,
$$
\begin{aligned}
x_{n+1} &= x_n - \frac{f(x_n)}{f'(x_n)} \\
&= x_n - \frac{x_n^{\frac{1}{k}}}{\frac{1}{k} x_n^{\frac{1}{k} - 1}} \\
&= x_n - \frac{kx_n^{\frac{1}{k}}}{x_n^{\frac{1}{k} - 1}} \\
&= x_n - kx_n = (1-k)x_n \\
\end{aligned}
$$
