# 3940 AS08

## Main

### Question 1

From the question, we have
$$
\begin{aligned}
x_1 &= g_1(x_1, x_2) = \frac{1}{\sqrt{5}}x_2 \\
x_2 &= g_2(x_1, x_2) = \frac{1}{4}(\sin x_1 + \cos x_2)
\end{aligned}
$$
Since 
$$
\begin{aligned}
\frac{\partial g_1}{\partial x_1} &= 0 \\
\frac{\partial g_2}{\partial x_1} &= \frac{1}{4}\cos x_1 \\
\frac{\partial g_1}{\partial x_1} &= \frac{1}{\sqrt{5}} \\
\frac{\partial g_2}{\partial x_2} &= -\frac{1}{4}\sin x_2 \\
\end{aligned}
$$
Therefore, in domain $D = \left\{ (x_1, x_2)' | 0\leq x_1,x_2 \leq 1  \right\}$
$$
\begin{aligned}
|\frac{\partial g_1}{\partial x_1}| &= 0 \\
|\frac{\partial g_2}{\partial x_1}| &\leq \frac{1}{4} \\
|\frac{\partial g_1}{\partial x_1}| &= \frac{1}{\sqrt{5}} \\
|\frac{\partial g_2}{\partial x_2}| &\leq -\frac{1}{4} \\
\end{aligned}
$$


So, $|\frac{\partial g_i}{\partial x_j}| &\leq \frac{K}{2} \\$

**Therefore, the mapping has a unique fixed point. (a)**

According to the fixed-point iteration
$$
x_1^k = \frac{1}{\sqrt{5}}\{x_2^{k-1}\} \\
x_2^k = \frac{1}{4}\{\sin{x_1^{k-1}} + \cos x_2^{k-1}\}
$$
Consider the initial guessed solutions as
$$
x_1^0 = 0.25, x_2^0 = 0.25
$$
Consider the iteration steps with tolerance $10^{-5}$ that is $||x^k - x^{k-1}|| \leq 10^{-5}$

![image-20211215164517979](../../../Users/WendellWang/AppData/Roaming/Typora/typora-user-images/image-20211215164517979.png)

**Hence, the solution of the non-linear equation is $x_1 = 0.12124, x_2 = 0.27111$ (b)**

According to the Gauss Seidel acceleration method,
$$
x_1^k = \frac{1}{\sqrt{5}}\{x^{k-1}_2\} \\
x_2^k = \frac{1}{4}\{\sin x_1^k + \cos x_2^{k-1}\}
$$
Consider the initial guessed solution as 
$$
x_1^0 = 0.25, x_2^0 = 0.25
$$
So,

![image-20211215164822559](../../../Users/WendellWang/AppData/Roaming/Typora/typora-user-images/image-20211215164822559.png)

**Therefore, the solution of the non-linear equation is $x_1 = 0.12124, x_2 = 0.271111$ (c)**

### Question 2

The nonlinear system of the equations are 
$$
\begin{aligned}
3x_1^2 - x_2^2 &= 0 \\
3x_1x_2^2 - x_1^3 - 1 &= 0
\end{aligned}
$$
 The Jacobean matrix is
$$
J(x) = \begin{pmatrix}6x_1 & -2x_2 \\ 3x^2_2 - 3x^2_1 & 6x_1x_2\end{pmatrix}
$$
and $x^{(0) = (1,1)^t}$

So,
$$
\begin{aligned}
F(x^{(0)}) &= (2,1)^t \\
A_0 &= J(x^0) \\
&= \begin{pmatrix}6 & -2 \\ 0 & 6\end{pmatrix}\\
\end{aligned}
$$
Solving the linear system,
$$
\begin{aligned}

J(x^{(0)})y^{(0)} &= -F(x^{(0)}) \\
y^{(0)} &= -J(x^{(0)})^{-1}F(x^{(0)}) \\
&= -\begin{bmatrix}6 & -2 \\ 0 & 6\end{bmatrix}^{-1}\begin{bmatrix}2 \\ 1\end{bmatrix} \\
&= \begin{bmatrix}-0.39 \\ -0.17\end{bmatrix}

\end{aligned}
$$
Now,
$$
y_1 = F[x^{(0)}]-F[x^{(0)}] = \begin{bmatrix}-1.5726 \\ -0.9663 \end{bmatrix} \\
s_1 = x^{(1)} - x^{(0)} = \begin{bmatrix} -0.39 \\ -0.17 \end{bmatrix}
$$
So that
$$
[A_1]^{-1} = [A_0]^{-1} + [(s_1' - A_0^{-1}y_1)s_1'A_0^{-1}] = \begin{bmatrix} 0.238271 & .130749 \\ -0.074858 & .288279\end{bmatrix}
$$
and 
$$
x^{(2)} = x^{(1)} - [A_1]^{-1}F(x^{(1)}) = \begin{bmatrix}.50333 \\ .8523\end{bmatrix}
$$


### Question 3

$$
\begin{aligned}
g(x_1, x_2) &= \cos (x_1 + x_2) + \sin x_1 \cos x_2 \\
\frac{\partial g}{\partial x_1 } &= -\sin (x_1 + x_2) + \cos x_1 = 0\\
\frac{\partial g}{\partial x_2 } &= -\sin (x_1 + x_2) - \sin x_2 = 0\\
\Delta g &= (-\sin (x_1 + x_2) + \cos x_i)i + (-\sin(x_1 + x_2)-\sin x_2)j
\end{aligned}
$$



### Question 4



### Question 5

